Assignment 9 Answers:

### Question 1

Prove by induction that 1 + 5 + 9 + ... + (4n-3) = n(2n-1)

	n=1
	
	1 = 1(2(1) - 1)
	
	1 = 1(2-1)
	
	1 = 1(1)
	
	1 = 2-1
	
	Base case is true.

	k(2k-1) + (4(k+1)-3) = (k+1)(2(k+1)-1)
	
	(2k^2-k) + (4k+4-3) = (k+1)(2k+2-1)
	
	2k^2-k+4k+1 = (k+1)(2k+1)
	
	2k^2+3k+1 = 2k^2+k+2k+1
	
	Answer: 2k^2+3k+1 = 2k^2+3k+1

### Question 2

n^3 + 2n = 3m

	n=1

	1 = (1^3 + 2(1)) / 3

	1 = (1 + 2) / 3

	1 = 3 / 3

	1 = 1

	Base case is true

	n^3 = 3m -2n

	(n+1)^3 + 2(n+1) = 3m

	(n+1)(n+1)(n+1) + (2n+2) = 3m

	(n^2+n+n+1)(n+1) + (2n+2) = 3m

	(n^2+2n+1)(n+1) + (2n+2) = 3m

	(n^3+n^2+2n^2+2n+n+1) + (2n+2) = 3m

	(n^3+3n^2+3n+1) + (2n+2) = 3m

	n^3+3n^2+5n+3 = 3m

	(3m-2n)+3n^2+5n+3 = 3m

	3m+3n^2+3n+3 = 3m

	3(m+n^2+n+1) = 3m

	Answer: 3m = 3m

### Question 3	

9^n - 1 = 8m

	n=1

	9^1 - 1 = 8m

	9 - 1 = 8m

	8 = 8m

	m=1

	8 = 8(1)

	8 = 8

	Base case is true

	9^n = 8m

	9^(n+1) - 1 = 8m

	9^n * 9 - 1 = 8m

	8m * 9 - 1 = 8m

	8m * 8 = 8m

	8(m * 1) = 8m

	Answer: 8m = 8m
